Add a funny corner case, we handle it well

test/issue-related/issue38_test.c
@@ -3,3 +3,18 @@
 struct foo {
 	int left;
 };
+
+
+/* This is a funny corner case, that works.
+   The internal struct declaration does not
+   defined any field for foo2, but defines a new
+   struct type. */
+struct foo2 {
+	int left;
+	struct xy {
+		int x;
+		int y;
+	};
+};
+
+struct xy bar(void);
