test/snapshots/Issue38_test.fst
@@ -66,3 +66,135 @@ requires exists* (y: foo). (x |-> y) **
 (y.left |-> a0)
 ensures exists* w. foo_pred x w ** pure (w == {left = a0})
 {fold foo_pred x ({left = a0}) }
+
+noeq
+type foo2 = {
+left: ref Int32.t;
+}
+
+[@@erasable]
+noeq
+type foo2_spec = {
+left : Int32.t
+
+}
+
+let foo2_pred ([@@@mkey]x:ref foo2) (s:foo2_spec) : slprop =
+exists* (y: foo2). (x |-> y) **
+(y.left |-> s.left)
+
+assume val foo2_spec_default : foo2_spec
+
+assume val foo2_default (foo2_var_spec:foo2_spec) : foo2
+
+ghost
+fn foo2_pack (foo2_var:ref foo2) (#foo2_var_spec:foo2_spec)
+requires foo2_var|-> foo2_default foo2_var_spec
+ensures exists* v. foo2_pred foo2_var v ** pure (v == foo2_var_spec)
+{ admit() }
+
+ghost
+fn foo2_unpack (foo2_var:ref foo2)
+requires exists* v. foo2_pred foo2_var v 
+ensures exists* u. foo2_var |-> u
+{ admit() }
+
+fn foo2_alloc ()
+returns x:ref foo2
+ensures freeable x
+ensures exists* v. foo2_pred x v
+{ admit () }
+
+fn foo2_free (x:ref foo2)
+requires freeable x
+requires exists* v. foo2_pred x v
+{ admit() }
+
+
+ghost fn foo2_explode (x:ref foo2) (#s:foo2_spec)
+requires foo2_pred x s
+ensures exists* (v: foo2). (x |-> v) ** (v.left |-> s.left)
+
+{unfold foo2_pred}
+
+
+ghost
+fn foo2_recover (x:ref foo2) (#a0 : Int32.t)
+
+requires exists* (y: foo2). (x |-> y) ** 
+(y.left |-> a0)
+ensures exists* w. foo2_pred x w ** pure (w == {left = a0})
+{fold foo2_pred x ({left = a0}) }
+
+noeq
+type xy = {
+x: ref Int32.t;
+y: ref Int32.t;
+}
+
+[@@erasable]
+noeq
+type xy_spec = {
+x : Int32.t;
+y : Int32.t
+
+}
+
+let xy_pred ([@@@mkey]x:ref xy) (s:xy_spec) : slprop =
+exists* (y: xy). (x |-> y) **
+(y.x |-> s.x) **
+(y.y |-> s.y)
+
+assume val xy_spec_default : xy_spec
+
+assume val xy_default (xy_var_spec:xy_spec) : xy
+
+ghost
+fn xy_pack (xy_var:ref xy) (#xy_var_spec:xy_spec)
+requires xy_var|-> xy_default xy_var_spec
+ensures exists* v. xy_pred xy_var v ** pure (v == xy_var_spec)
+{ admit() }
+
+ghost
+fn xy_unpack (xy_var:ref xy)
+requires exists* v. xy_pred xy_var v 
+ensures exists* u. xy_var |-> u
+{ admit() }
+
+fn xy_alloc ()
+returns x:ref xy
+ensures freeable x
+ensures exists* v. xy_pred x v
+{ admit () }
+
+fn xy_free (x:ref xy)
+requires freeable x
+requires exists* v. xy_pred x v
+{ admit() }
+
+
+ghost fn xy_explode (x:ref xy) (#s:xy_spec)
+requires xy_pred x s
+ensures exists* (v: xy). (x |-> v) ** (v.x |-> s.x) ** 
+(v.y |-> s.y)
+
+{unfold xy_pred}
+
+
+ghost
+fn xy_recover (x:ref xy) (#a0 : Int32.t)
+(#a1 : Int32.t)
+
+requires exists* (y: xy). (x |-> y) ** 
+(y.x |-> a0) **
+(y.y |-> a1)
+ensures exists* w. xy_pred x w ** pure (w == {x = a0;
+y = a1})
+{fold xy_pred x ({x = a0;
+y = a1}) }
+
+fn bar_decl ()
+returns xy
+{
+admit();
+}
